fix dispatcher spec and init_dispatcher impl to save the full context
other references to dispatcher impl are broken at present

verified/pagedb.s.dfy
@@ -120,7 +120,8 @@ lemma validPageDbImpliesWellFormed(d:PageDb)
 
 predicate validDispatcherContext(dc:DispatcherContext)
 {
-    R4 in dc.regs && R5  in dc.regs && R6  in dc.regs && R7  in dc.regs
+    R0 in dc.regs && R1 in dc.regs && R2 in dc.regs && R3 in dc.regs
+    && R4  in dc.regs && R5  in dc.regs && R6  in dc.regs && R7  in dc.regs
     && R8  in dc.regs && R9  in dc.regs && R10 in dc.regs && R11 in dc.regs
     && R12 in dc.regs && LR(User) in dc.regs && SP(User) in dc.regs
     && decode_mode'(psr_mask_mode(dc.cpsr)) == Just(User)
